refactor: split modal logic details to another module

KripkeGameAnalysis/Basic.lean
@@ -1,100 +1,5 @@
-import Mathlib.Data.Finset.Basic
-import Mathlib.Data.Finset.Defs
-import Mathlib.Data.Finset.Dedup
-import Mathlib.Data.Finset.Prod
-import Mathlib.Data.Finset.Powerset
-import Mathlib.Data.Fintype.Basic
-import Mathlib.Data.Fintype.Card
-
-import KripkeGameAnalysis.GenericExtras.FinsetEquivCharacteristic
-
-inductive ModalFormula (vars : Type) : Type where
-| var : vars → ModalFormula vars
-| neg : ModalFormula vars → ModalFormula vars
-| and : ModalFormula vars → ModalFormula vars → ModalFormula vars
-| box : ModalFormula vars → ModalFormula vars
-
-namespace ModalFormula
-  variable {vars : Type}
-
-  abbrev not := fun (φ: ModalFormula vars) => neg φ
-  abbrev or := fun (φ1 φ2: ModalFormula vars) => not (and (not φ1) (not φ2))
-  abbrev implies := fun (φ1 φ2: ModalFormula vars) => or (not φ1) φ2
-  abbrev dia := fun (φ: ModalFormula vars) => not (box (not φ))
-end ModalFormula
-
-def KripkeFrame (vertices : Type) : Type := vertices → vertices → Bool
-namespace KripkeFrame
-  def vertices (_ : KripkeFrame v) : Type := v
-  def accessible (frame : KripkeFrame v) (i j : frame.vertices) : Bool := frame i j
-
-  def Valuation (frame : KripkeFrame v) (vars : Type) : Type := vars → frame.vertices → Bool
-
-  def Valuation.decideSatisfaction {frame : KripkeFrame v} [Fintype frame.vertices]
-                                   (i : frame.vertices) (fml : ModalFormula vars) (val : frame.Valuation vars) : Bool :=
-  match fml with
-    | ModalFormula.var x => val x i
-    | ModalFormula.neg φ => !(val.decideSatisfaction i φ)
-    | ModalFormula.and φ1 φ2 => val.decideSatisfaction i φ1 && val.decideSatisfaction i φ2
-    | ModalFormula.box φ => decide (∀j: frame.vertices, if frame.accessible i j then val.decideSatisfaction j φ else true)
-
-end KripkeFrame
-
-/-- A Kripke frame of `frameSize` possible worlds is a directed graph with `frameSize` vertices.
-
-We think of the vertices in the graph as being numbered from `0` to `frameSize - 1`, inclusive,
-and we think the `j`-th vertex is accessible from the `i`-th vertex if and only if there is an edge from `i` to `j`.
-
-The graph, then, is represented by a function that takes two natural numbers `n` and `m` as input,
-and returns `true` if there is an edge from vertex `n` to vertex `m`, and `false` otherwise.
--/
-def FiniteKripkeFrame (frameSize : Nat) : Type := KripkeFrame (Fin frameSize)
-namespace FiniteKripkeFrame
-  instance (frame : FiniteKripkeFrame n) : Fintype frame.vertices := inferInstanceAs (Fintype (Fin n))
-  instance (frame : FiniteKripkeFrame n) : DecidableEq frame.vertices := inferInstanceAs (DecidableEq (Fin n))
-
-  def allNodes (frame : FiniteKripkeFrame n) : Finset frame.vertices := Finset.univ
-  lemma allNodes_card_eq_frameSize (frame : FiniteKripkeFrame n) : frame.allNodes.card = n :=
-    by apply Fintype.card_fin
-
-  def accessibilityRelationCount (frame : FiniteKripkeFrame n) : ℕ :=
-    ((frame.allNodes.product (frame.allNodes)).filter (fun a => frame.accessible a.fst a.snd)).card
-
-  structure FiniteValuation (frame : FiniteKripkeFrame n) (vars : Type) [Fintype vars] [DecidableEq vars] where
-    valuation : frame.Valuation vars
-
-  namespace FiniteValuation
-    def equivToFinSetRepresentation {finVars : Type} {frame : FiniteKripkeFrame n} [Fintype finVars] [DecidableEq finVars]:
-                                    (frame.FiniteValuation finVars) ≃ (Finset (finVars × frame.vertices)) :=
-      let valPowersetEquiv : (frame.Valuation finVars) ≃ (Finset (finVars × frame.vertices)) := finsetProdEquivCurriedCharacteristic.symm
-      let valEquiv : (frame.FiniteValuation finVars) ≃ (frame.Valuation finVars) := {
-        toFun := fun val => val.valuation,
-        invFun := fun val => { valuation := val },
-        left_inv := by intro val; simp,
-        right_inv := by intro val; simp
-      }
-      valEquiv.trans valPowersetEquiv
-  end FiniteValuation
-
-  def allValuations (frame : FiniteKripkeFrame n) (finVars : Type) [varsFin : Fintype finVars] [DecidableEq finVars] : Finset (frame.FiniteValuation finVars) :=
-    let valuationsAsPsets := (Finset.product varsFin.elems frame.allNodes).powerset
-    valuationsAsPsets.map ((@FiniteValuation.equivToFinSetRepresentation _ _ frame).symm.toEmbedding)
-
-  def satisfiesForAllValuations {frame : FiniteKripkeFrame n} (finVars : Type) [Fintype finVars] [DecidableEq finVars]
-                                (i : frame.vertices) (fml : ModalFormula finVars) : Bool :=
-    decide (∀finval ∈ frame.allValuations finVars, finval.valuation.decideSatisfaction i fml)
-
-  def countSatisfyingNodes (frame : FiniteKripkeFrame n)
-                           (fml : ModalFormula finVars) [Fintype finVars] [DecidableEq finVars] : ℕ :=
-    (frame.allNodes.filter (fun i => satisfiesForAllValuations finVars i fml)).card
-
-  lemma countSatisfyingNodes_leq_frameSize
-    (frame : FiniteKripkeFrame n) (fml : ModalFormula finVars)
-    [Fintype finVars] [DecidableEq finVars]: frame.countSatisfyingNodes fml ≤ n := by
-    simp only [FiniteKripkeFrame.countSatisfyingNodes]
-    simp only [← frame.allNodes_card_eq_frameSize]
-    apply Finset.card_filter_le
-end FiniteKripkeFrame
+import KripkeGameAnalysis.ModalLogic.Basic
+import KripkeGameAnalysis.GenericExtras.Fintype
 
 inductive KripkeGameVars : Type
 | p
@@ -104,8 +9,7 @@ inductive KripkeGameVars : Type
 deriving Ord, BEq, DecidableEq
 
 instance KripkeGameVars.fintype : Fintype KripkeGameVars :=
-  open KripkeGameVars in
-  ⟨⟨{p, q, r, s}, by simp⟩, fun x => by cases x <;> simp⟩
+  open KripkeGameVars in ⟨⟨{p, q, r, s}, by simp⟩, fun x => by cases x <;> simp⟩
 
 def KripkeGameVars.all : Finset KripkeGameVars := Finset.univ
 
@@ -122,19 +26,11 @@ structure KripkeGameVisibleState where
   queriesAndAnswers : List ((ModalFormula KripkeGameVars) × Fin (frameSize + 1))
 
 namespace KripkeGameVisibleState
-  def allPossibleInitialVisibleStates : Finset KripkeGameVisibleState :=
-    let frameSize := 4
-    let maxRelSize := frameSize * frameSize
-    let mapRelSizeToState := fun (n : Fin (maxRelSize + 1)) =>
-      {
-        frameSize := frameSize,
-        accessiblityRelationSize := n,
-        queriesAndAnswers := []
-        : KripkeGameVisibleState
-      }
-    let mappingInjective: Function.Injective mapRelSizeToState := by
-      intro n1 n2 h; simp only [mapRelSizeToState] at h; injection h
-    (Finset.univ : Finset (Fin (4 * 4 + 1))).map ⟨mapRelSizeToState, mappingInjective⟩
+  -- An initial visible state should have a frame size of 4, and an empty query-answer list.
+  def InitialVisibleState : Type :=
+   { state : KripkeGameVisibleState // state.frameSize = 4 ∧ state.queriesAndAnswers = [] }
+
+  instance : Fintype InitialVisibleState := sorry
 
   def withNewQueryAndAnswer (state : KripkeGameVisibleState) (query : ModalFormula KripkeGameVars) (answer : Fin (state.frameSize + 1)) : KripkeGameVisibleState :=
     { state with queriesAndAnswers := (query, answer) :: state.queriesAndAnswers }
@@ -151,6 +47,6 @@ namespace KripkeGameVisibleState
                   WinningStrategy (n + 1) state
 end KripkeGameVisibleState
 
-def kripkeGame_winning_strategy : ∀state ∈ KripkeGameVisibleState.allPossibleInitialVisibleStates,
-                                  KripkeGameVisibleState.WinningStrategy 10 state :=
+def kripkeGame_winning_strategy : ∀state : KripkeGameVisibleState.InitialVisibleState,
+                                  KripkeGameVisibleState.WinningStrategy 10 state.val :=
   sorry
