KripkeGameAnalysis/ModalLogic/Basic.lean
@@ -1,0 +1,98 @@
+import Mathlib.Data.Finset.Basic
+import Mathlib.Data.Finset.Defs
+import Mathlib.Data.Finset.Dedup
+import Mathlib.Data.Finset.Prod
+import Mathlib.Data.Finset.Powerset
+import Mathlib.Data.Fintype.Basic
+import Mathlib.Data.Fintype.Card
+
+import KripkeGameAnalysis.GenericExtras.FinsetEquivCharacteristic
+
+inductive ModalFormula (vars : Type) : Type where
+| var : vars → ModalFormula vars
+| neg : ModalFormula vars → ModalFormula vars
+| and : ModalFormula vars → ModalFormula vars → ModalFormula vars
+| box : ModalFormula vars → ModalFormula vars
+
+namespace ModalFormula
+  variable {vars : Type}
+
+  abbrev not := fun (φ: ModalFormula vars) => neg φ
+  abbrev or := fun (φ1 φ2: ModalFormula vars) => not (and (not φ1) (not φ2))
+  abbrev implies := fun (φ1 φ2: ModalFormula vars) => or (not φ1) φ2
+  abbrev dia := fun (φ: ModalFormula vars) => not (box (not φ))
+end ModalFormula
+
+/-- A Kripke frame is a directed graph.
+
+The graph is represented by a function that takes two vertices `i` and `j` as input,
+and returns `true` if there is an edge from vertex `i` to vertex `j`, and `false` otherwise.
+-/
+def KripkeFrame (vertices : Type) : Type := vertices → vertices → Bool
+namespace KripkeFrame
+  def vertices (_ : KripkeFrame v) : Type := v
+  def accessible (frame : KripkeFrame v) (i j : frame.vertices) : Bool := frame i j
+
+  def Valuation (frame : KripkeFrame v) (vars : Type) : Type := vars → frame.vertices → Bool
+
+  def Valuation.decideSatisfaction {frame : KripkeFrame v} [Fintype frame.vertices]
+                                   (i : frame.vertices) (fml : ModalFormula vars) (val : frame.Valuation vars) : Bool :=
+  match fml with
+    | ModalFormula.var x => val x i
+    | ModalFormula.neg φ => !(val.decideSatisfaction i φ)
+    | ModalFormula.and φ1 φ2 => val.decideSatisfaction i φ1 && val.decideSatisfaction i φ2
+    | ModalFormula.box φ => decide (∀j: frame.vertices, if frame.accessible i j then val.decideSatisfaction j φ else true)
+
+end KripkeFrame
+
+/--
+A finite Kripke frame is a Kripke frame with a finite number of vertices.
+We think of the vertices in the Kripke frame as being numbered from `0` to `frameSize - 1`, inclusive.
+-/
+def FiniteKripkeFrame (frameSize : Nat) : Type := KripkeFrame (Fin frameSize)
+namespace FiniteKripkeFrame
+  instance (frame : FiniteKripkeFrame n) : Fintype frame.vertices := inferInstanceAs (Fintype (Fin n))
+  instance (frame : FiniteKripkeFrame n) : DecidableEq frame.vertices := inferInstanceAs (DecidableEq (Fin n))
+
+  def allNodes (frame : FiniteKripkeFrame n) : Finset frame.vertices := Finset.univ
+  lemma allNodes_card_eq_frameSize (frame : FiniteKripkeFrame n) : frame.allNodes.card = n :=
+    by apply Fintype.card_fin
+
+  def accessibilityRelationCount (frame : FiniteKripkeFrame n) : ℕ :=
+    ((frame.allNodes.product (frame.allNodes)).filter (fun a => frame.accessible a.fst a.snd)).card
+
+  structure FiniteValuation (frame : FiniteKripkeFrame n) (vars : Type) [Fintype vars] [DecidableEq vars] where
+    valuation : frame.Valuation vars
+
+  namespace FiniteValuation
+    def equivToFinSetRepresentation {finVars : Type} {frame : FiniteKripkeFrame n} [Fintype finVars] [DecidableEq finVars]:
+                                    (frame.FiniteValuation finVars) ≃ (Finset (finVars × frame.vertices)) :=
+      let valPowersetEquiv : (frame.Valuation finVars) ≃ (Finset (finVars × frame.vertices)) := finsetProdEquivCurriedCharacteristic.symm
+      let valEquiv : (frame.FiniteValuation finVars) ≃ (frame.Valuation finVars) := {
+        toFun := fun val => val.valuation,
+        invFun := fun val => { valuation := val },
+        left_inv := by intro val; simp,
+        right_inv := by intro val; simp
+      }
+      valEquiv.trans valPowersetEquiv
+  end FiniteValuation
+
+  def allValuations (frame : FiniteKripkeFrame n) (finVars : Type) [varsFin : Fintype finVars] [DecidableEq finVars] : Finset (frame.FiniteValuation finVars) :=
+    let valuationsAsPsets := (Finset.product varsFin.elems frame.allNodes).powerset
+    valuationsAsPsets.map ((@FiniteValuation.equivToFinSetRepresentation _ _ frame).symm.toEmbedding)
+
+  def satisfiesForAllValuations {frame : FiniteKripkeFrame n} (finVars : Type) [Fintype finVars] [DecidableEq finVars]
+                                (i : frame.vertices) (fml : ModalFormula finVars) : Bool :=
+    decide (∀finval ∈ frame.allValuations finVars, finval.valuation.decideSatisfaction i fml)
+
+  def countSatisfyingNodes (frame : FiniteKripkeFrame n)
+                           (fml : ModalFormula finVars) [Fintype finVars] [DecidableEq finVars] : ℕ :=
+    (frame.allNodes.filter (fun i => satisfiesForAllValuations finVars i fml)).card
+
+  lemma countSatisfyingNodes_leq_frameSize
+    (frame : FiniteKripkeFrame n) (fml : ModalFormula finVars)
+    [Fintype finVars] [DecidableEq finVars]: frame.countSatisfyingNodes fml ≤ n := by
+    simp only [FiniteKripkeFrame.countSatisfyingNodes]
+    simp only [← frame.allNodes_card_eq_frameSize]
+    apply Finset.card_filter_le
+end FiniteKripkeFrame
